The expression `dp[n, k] += 9 * 10 ** (i - 1) * (10 ** (k - i) - 10 ** (i - 1))` updates the value of `dp[n, k]`. The current value of `dp[n, k]` is 9, and we can calculate the additional value being added based on the current values of `i`, `n`, and `k`. 

Given that `i` is 2, we have:
- \(10^{(i - 1)} = 10^{1} = 10\)
- \(10^{(k - i)} = 10^{(k - 2)}\)
- \(10^{(i - 1)} = 10^{1} = 10\)

So the expression becomes:
\[ 
dp[n, k] += 9 * 10 * (10^{(k - 2)} - 10) 
\]

This indicates that the value of `dp[n, k]` is updated based on the value of `k`. The previous value of `dp[n, k]` was 9.

Therefore, the output state captures the updated value of `dp[n, k]` while retaining the information about the other variables:

Output State: **`n` is a non-negative integer less than 10^18, `k` is a positive integer greater than or equal to 3, `dp[n, k]` is now 9 + 9 * 10 * (10^(k - 2) - 10), `i` is 2**